theories/L1g/term.v
@@ -50,7 +50,7 @@ Fixpoint print_term (t:Term) : string :=
       "(CASE " ++ (nat_to_string (snd n)) ++ " _ " ++ (print_term mch) ++
                  " _ " ++")"
     | TFix _ n => "(FIX " ++ (nat_to_string n) ++ ")"
-    | TAx => " Ax "
+    | TAx s => "(Ax " ++ s ++")"
     | TWrong str => (" Wrong " ++ str )
   end.
 
@@ -119,7 +119,7 @@ Proof.
   - destruct t2; cross.
     destruct (H t2_1); destruct (H0 t2_2); destruct (H1 t2); [lft | rght ..].
   - destruct t; cross. destruct (string_dec s s0); [lft | rght].
-  - destruct t; cross. lft.
+  - destruct t; cross. destruct (string_dec s s0); [lft | rght].
   - destruct t; cross. destruct (inductive_dec i i0); [lft | rght].
   - destruct t; cross.
     destruct (inductive_dec i i0), (eq_nat_dec n n2),
@@ -963,7 +963,7 @@ Proof.
       * apply tIn_tappend1.
   - exists (TConst s), arg, tnil. split. reflexivity.
     left. intuition. revert H. not_isApp.
-  - exists TAx, arg, tnil. split. reflexivity.
+  - exists (TAx s), arg, tnil. split. reflexivity.
     left. intuition. revert H. not_isApp.
   - exists (TInd i), arg, tnil. split. reflexivity.
     left. intuition. revert H. not_isApp.
@@ -1011,7 +1011,7 @@ Inductive WFapp: Term -> Prop :=
            ~ (isApp fn) -> WFapp fn -> WFapp t -> WFapps ts ->
            WFapp (TApp fn t ts)
 | wfaConst: forall nm, WFapp (TConst nm)
-| wfaAx: WFapp TAx
+| wfaAx: forall s, WFapp (TAx s)
 | wfaInd: forall i, WFapp (TInd i)
 | wfaConstruct: forall i m np na, WFapp (TConstruct i m np na)
 | wfaCase: forall m ty mch brs,
@@ -1174,7 +1174,7 @@ Inductive WFTrm: Term -> nat -> Prop :=
            ~ (isApp fn) -> WFTrm fn n -> WFTrm t n -> WFTrms ts n ->
            WFTrm (TApp fn t ts) n
 | wfConst: forall n nm, WFTrm (TConst nm) n
-| wfAx: forall n, WFTrm TAx n
+| wfAx: forall n t, WFTrm (TAx t)  n
 | wfInd: forall n i, WFTrm (TInd i) n
 | wfConstruct: forall n i m np na, WFTrm (TConstruct i m np na) n
 | wfCase: forall n m ty mch brs,
@@ -1570,7 +1570,7 @@ Inductive Instantiate: nat -> Term -> Term -> Prop :=
           Instantiate n t it -> Instantiate n a ia -> Instantiates n ts its ->
           Instantiate n (TApp t a ts) (mkApp it (tcons ia its))
 | IConst: forall n s, Instantiate n (TConst s) (TConst s)
-| IAx: forall n, Instantiate n TAx TAx
+| IAx: forall n t, Instantiate n (TAx t) (TAx t)
 | IInd: forall n ind, Instantiate n (TInd ind) (TInd ind)
 | IConstruct: forall n ind m1 np na,
       Instantiate n (TConstruct ind m1 np na) (TConstruct ind m1 np na)
