theories/L1g/test_wcbvEval.v
@@ -718,6 +718,19 @@ Goal
   vm_compute. reflexivity.
 Qed.
 
+Require Import Benchmarks.vs.
+
+(****** runs out of space **************
+Time Quote Recursively Definition p_myMain := vs.myMain.
+Time Definition P_myMain :=
+  Eval vm_compute in (L1g.compile.program_Program p_myMain).
+Definition P_env_myMain := env P_myMain.
+Definition P_main_myMain := AstCommon.main P_myMain.
+Time Definition eval_myMain :=
+  Eval vm_compute in (wcbvEval P_env_myMain 4000 P_main_myMain).
+Set Printing Width 80.
+Print eval_myMain.
+************************)
 
 
 (********
